src/3d/prelude/Actions.fsti
@@ -408,21 +408,6 @@ val validate_string
   (terminator: t)
 : Tot (validate_with_action_t (parse_string p terminator) true_inv eloc_none false)
 
-inline_for_extraction noextract
-let dep_pair_no_terminator_validators
-  (#t: eqtype)
-  (#terminator: t)
-  (#nz: bool)
-  (#k: parser_kind nz)
-  (#pl: dep_pair_no_terminator_types terminator)
-  (f: dep_pair_no_terminator_parsers k pl)
-  (inv: slice_inv)
-  (l: eloc)
-  (allow_reading: bool)
-: Tot Type0
-=
-  (x: t { x <> terminator }) -> Tot (validate_with_action_t (f x) inv l allow_reading)
-
 inline_for_extraction
 noextract
 val validate_sized_list_dep_pair_with_terminator
@@ -438,13 +423,13 @@ val validate_sized_list_dep_pair_with_terminator
   (terminator: t)
   (#nzpl: bool)
   (#k: parser_kind nzpl)
-  (#pl: dep_pair_no_terminator_types terminator)
-  (#f: dep_pair_no_terminator_parsers k pl)
+  (#pl: t -> Tot Type0)
+  (#f: (x: t) -> Tot (parser k (pl x)))
   (#inv: slice_inv)
   (#l: eloc)
   (#allow_reading: bool)
-  (v: dep_pair_no_terminator_validators f inv l allow_reading)
-: Tot (validate_with_action_t (parse_sized_list_dep_pair_with_terminator n pt terminator pl f) (conj_inv invt inv) (lt `eloc_union` l) false)
+  (v: (x: t) -> Tot (validator (f x)))
+: Tot (validate_with_action_t (parse_sized_list_dep_pair_with_terminator n pt terminator f) (conj_inv invt inv) (lt `eloc_union` l) false)
 
 ////////////////////////////////////////////////////////////////////////////////
 
